remove case left and right labels

theory/Runtime_Semantics.thy
@@ -5,8 +5,6 @@ begin
 datatype control_label = 
   L_Seq var ("`_" [71] 70) | 
   L_Spawn var ("._" [71] 70) |
-  L_Left var ("\<upharpoonleft>\<bar>_" [71] 70) |
-  L_Right var ("\<upharpoonleft>:_" [71] 70) | 
   L_Up var ("\<upharpoonleft>_" [71] 70) |
   L_Down var ("\<downharpoonleft>_" [71] 70)
 
@@ -60,6 +58,22 @@ inductive seq_step :: "state \<Rightarrow> state \<Rightarrow> bool" (infix "\<h
     \<rbrakk> \<Longrightarrow>
     \<langle>LET x = SND x\<^sub>p in e; \<rho>; \<kappa>\<rangle> \<hookrightarrow> \<langle>e; \<rho> ++ [x \<mapsto> \<omega>]; \<kappa>\<rangle>
   " |
+  Case_Left: "
+    \<lbrakk> 
+      \<rho> x\<^sub>s = Some \<lbrace>Left x\<^sub>l', \<rho>\<^sub>l\<rbrace>; 
+      \<rho>\<^sub>l x\<^sub>l' = Some \<omega>\<^sub>l
+    \<rbrakk> \<Longrightarrow>
+    \<langle>LET x = CASE x\<^sub>s LEFT x\<^sub>l |> e\<^sub>l RIGHT x\<^sub>r |> e\<^sub>r in e; \<rho>; \<kappa>\<rangle> \<hookrightarrow> 
+    \<langle>e\<^sub>l; \<rho> ++ [x\<^sub>l \<mapsto> \<omega>\<^sub>l]; \<langle>x, e, \<rho>\<rangle> # \<kappa>\<rangle>
+  " |
+  Case_Right: "
+    \<lbrakk>
+      \<rho> x\<^sub>s = Some \<lbrace>Right x\<^sub>r', \<rho>\<^sub>r\<rbrace>; 
+      \<rho>\<^sub>r x\<^sub>r' = Some \<omega>\<^sub>r
+    \<rbrakk> \<Longrightarrow>
+    \<langle>LET x = CASE x\<^sub>s LEFT x\<^sub>l |> e\<^sub>l RIGHT x\<^sub>r |> e\<^sub>r in e; \<rho>; \<kappa>\<rangle> \<hookrightarrow> 
+    \<langle>e\<^sub>r; \<rho> ++ [x\<^sub>r \<mapsto> \<omega>\<^sub>r]; \<langle>x, e, \<rho>\<rangle> # \<kappa>\<rangle>
+  " |
   Let_App: "
     \<lbrakk>
       \<rho> f = Some \<lbrace>Abs f\<^sub>l x\<^sub>l e\<^sub>l, \<rho>\<^sub>l\<rbrace> ; 
@@ -93,6 +107,7 @@ inductive concur_step :: "state_pool \<Rightarrow> state_pool \<Rightarrow> bool
     \<rbrakk> \<Longrightarrow>
     \<E> \<rightarrow> \<E> ++ [\<pi>;;\<downharpoonleft>x\<^sub>\<kappa> \<mapsto> \<sigma>']
   " |
+(*
   Seq_Step_Left: "
     \<lbrakk> 
       leaf \<E> \<pi> ;
@@ -111,11 +126,12 @@ inductive concur_step :: "state_pool \<Rightarrow> state_pool \<Rightarrow> bool
     \<rbrakk> \<Longrightarrow>
     \<E> \<rightarrow> \<E> ++ [\<pi>;;\<upharpoonleft>:x \<mapsto> \<langle>e\<^sub>r; \<rho> ++ [x\<^sub>r \<mapsto> \<omega>\<^sub>r]; \<langle>x, e, \<rho>\<rangle> # \<kappa>\<rangle>]
   " |
+*)
   Seq_Step_Up: "
     \<lbrakk> 
       leaf \<E> \<pi> ;
-      \<E> \<pi> = Some (\<langle>LET x = APP f x\<^sub>a in e; \<rho>; \<kappa>\<rangle>) ;
-      \<langle>LET x = APP f x\<^sub>a  in e; \<rho>; \<kappa>\<rangle> \<hookrightarrow> \<langle>e'; \<rho>'; \<langle>x, e, \<rho>\<rangle> # \<kappa>\<rangle>
+      \<E> \<pi> = Some (\<langle>LET x = b in e; \<rho>; \<kappa>\<rangle>) ;
+      \<langle>LET x = b  in e; \<rho>; \<kappa>\<rangle> \<hookrightarrow> \<langle>e'; \<rho>'; \<langle>x, e, \<rho>\<rangle> # \<kappa>\<rangle>
     \<rbrakk> \<Longrightarrow>
     \<E> \<rightarrow> \<E> ++ [\<pi>;;\<upharpoonleft>x \<mapsto> \<langle>e'; \<rho>'; \<langle>x, e, \<rho>\<rangle> # \<kappa>\<rangle>]
   " |
@@ -185,14 +201,6 @@ inductive path_balanced :: "control_path \<Rightarrow> bool" ("\<downharpoonrigh
   Linear[simp]: "
     \<downharpoonright>[`x]\<upharpoonleft>
   " |
-  Left_Down[simp]: "
-    \<downharpoonright>\<pi>\<upharpoonleft> \<Longrightarrow>
-    \<downharpoonright> (\<upharpoonleft>\<bar>x # (\<pi> ;; \<downharpoonleft>x)) \<upharpoonleft>
-  " |
-  Right_Down[simp]: "
-    \<downharpoonright>\<pi>\<upharpoonleft> \<Longrightarrow>
-    \<downharpoonright> (\<upharpoonleft>:x # (\<pi> ;; \<downharpoonleft>x)) \<upharpoonleft>
-  " |
   Up_Down[simp]: "
     \<downharpoonright>\<pi>\<upharpoonleft> \<Longrightarrow>
     \<downharpoonright> (\<upharpoonleft>x # (\<pi> ;; \<downharpoonleft>x)) \<upharpoonleft>
@@ -207,17 +215,5 @@ lemma up_down_balanced[simp]: "
    \<downharpoonright>[\<upharpoonleft>x, \<downharpoonleft>x] \<upharpoonleft>
 "
 using Up_Down path_balanced.Empty by fastforce
-
-lemma left_down_balanced[simp]: "
-   \<downharpoonright>[\<upharpoonleft>\<bar>x, \<downharpoonleft>x] \<upharpoonleft>
-"
-using Left_Down path_balanced.Empty by fastforce
-
-lemma right_down_balanced[simp]: "
-   \<downharpoonright>[\<upharpoonleft>:x, \<downharpoonleft>x] \<upharpoonleft>
-"
-using Right_Down path_balanced.Empty by fastforce
-
-
 
 end
